---
layout: single
title: Appendix
katex: True
tags: Physics
authors: Henry
Hidden: true
toc: true
toc_label: "Appendix"
toc_sticky: true
permalink: /physics/Appendix/
header:
  teaser: /assets/images/Pgfplots.png
sidebar:
 nav: "Physics"
---

## KaTeX Promotion

In case you are confused about how I manage to write Math Equations in a website...
[Press Here]({% link _Jekyll/2022-05-19-Katex.markdown %})


## Appendix B

 - Used in my post about [HKDSE Physics]({% link _Physics/2022-12-25-HKDSE.markdown %})

**Proposition 1.2.1**: $$r^2 \dot{\theta} \equiv h=\frac{|\underline{L}|}{m}$$

**Proof**

Going back to Planar Polar Coordinates:

$$
\hat{r}=\cos (\theta) \hat{x}+\sin (\theta) \hat{y}, \quad \hat{\theta}=-\sin (\theta) \hat{x}+\cos (\theta) \hat{y} .
$$

By **Chain Rule**,

$$
\dot{\hat{r}}=\dot{\theta}[-\sin (\theta) \hat{x}+\cos (\theta) \hat{y}]=\dot{\theta} \hat{\theta}, \quad \dot{\hat{\theta}}=\dot{\theta}[-\cos (\theta) \hat{x}-\sin (\theta) \hat{y}]=-\dot{\theta} \hat{r} .
$$

And 

$$
\underline{\dot{r}}=\frac{d}{d t}(r \hat{r})=\dot{r} \hat{r}+r \dot{\hat{r}}=\dot{r} \hat{r}+r \dot{\theta} \hat{\theta}
$$

Further Differentiation yields:

$$
\begin{aligned}
\underline{\ddot{r}}=\frac{d}{d t}(\dot{r} \hat{r}+r \dot{\theta} \hat{\theta}) & =\ddot{r} \hat{r}+\dot{r} \dot{\hat{r}}+\dot{r} \dot{\theta} \hat{\theta}+r \ddot{\theta} \hat{\theta}+r \dot{\theta} \dot{\hat{\theta}} \\
& =\ddot{r} \hat{r}+\dot{r} \dot{\theta} \hat{\theta}+\dot{r} \dot{\theta} \hat{\theta}+r \ddot{\theta} \hat{\theta}-r \dot{\theta} \dot{\theta} \hat{r} \\
& =\left(\ddot{r}-r \dot{\theta}^2\right) \hat{r}+(2 \dot{r} \dot{\theta}+r \ddot{\theta}) \hat{\theta}
\end{aligned}
$$

Since the force is a central force, we have:

$$
m\left(\ddot{r}-r \dot{\theta}^2\right) \hat{r}+m(2 \dot{r} \dot{\theta}+r \ddot{\theta}) \hat{\theta}=F_r(r) \hat{r} .
$$

We can quickly identify two equations:

$$
\begin{aligned}
\ddot{r}-r \dot{\theta}^2 & =F_r(r) / m \\
2 \dot{r} \dot{\theta}+r \ddot{\theta} & =0 .
\end{aligned}
$$

From the second equation

$$
\frac{1}{r} \frac{d}{d t}\left(r^2 \dot{\theta}\right)=0 \quad \Longrightarrow \quad r^2 \dot{\theta} \equiv h=\text { const }
$$

$$
\underline{L}=\underline{r} \times \underline{p}=m r \hat{r} \times \underline{\dot{r}}=m r \hat{r} \times(\dot{r} \hat{r}+r \dot{\theta} \hat{\theta})=m r \hat{r} \times r \dot{\theta} \hat{\theta}=m r^2 \dot{\theta} \hat{n} \equiv m h \hat{n}
$$

Hence:

$$r^2 \dot{\theta} \equiv h=\frac{|\underline{L}|}{m}$$

$$\blacksquare$$

## Appendix C

 

Dimensional Analysis is one of the most *helpful* knowledge in Physics. You can immediately tell if an answer is correct or not using it. For example if we accidentally squared a term that contains dimensions, we can almost immediately identify the mistake. 

```bash
N.B.: Two objects with different units cannot be added
```

**Proposition 1.3**: $$\sin x$$ doesn't have any units

Proof: Consider the series expansion of $$\sin x$$, *i.e.*

$$ \sin x=x-\frac{x^3}{3 !}+\frac{x^5}{5 !}-\cdots=\sum_{k=0}^n \frac{(-1)^k x^{2 k+1}}{(2 k+1) !}$$

First note that $$x$$ cannot have any units, otherwise $$x-\frac{x^3}{3 !}+\frac{x^5}{5 !}-\cdots$$ won't have any physical sense, as discussed above. 

Therefore $$\frac{x^3}{3 !}$$ and $$\frac{x^5}{5 !}$$ will have the same units as $$x$$, *i.e.* no units, so as the preceding terms. Hence $$\sum_{k=0}^n \frac{(-1)^k x^{2 k+1}}{(2 k+1) !}$$ have no units, and hence $$\sin x$$ has no units $$\blacksquare$$

Note that dimensional analysis cannot ensure that your answer is correct; rather, it occasionally picks up errors, but this is already *extremely* useful.

## Appendix D


   - Used in my post about [Cosets and Lagrange's Theoremc]({% link _Physics/2023-03-05-CosetsandLagrange.markdown %})


### Lemma
 
**Claim:**
Let $$G$$ be a group. If $$g, h \in G$$, then

There exists (Existence) a unique element (Uniqueness) $$k \in G$$ such that $$k * g=h$$

**Proof:**
(Existence) Let $$k:=h * g^{-1}$$. Then
$$
k * g=\left(h * g^{-1}\right) * g=h *\left(g^{-1} * g\right)=h * e=h,
$$
Where we have used **associativity** of group axioms. Hence $$k$$ exists $$\blacksquare$$


(Uniqueness)
 Now suppose that $$k^{\prime} * g=h$$. Then
$$
k=h * g^{-1}=\left(k^{\prime} * g\right) * g^{-1}=k^{\prime} *\left(g * g^{-1}\right)=k^{\prime} * e=k^{\prime}
$$

hence $$k$$ is unique $$\blacksquare$$


Therefore there exists a unique element $$k \in G$$ such that $$k * g=h$$ $$\blacksquare$$

## Appendix E

Ellispes are a form of conic sections. 

Incomplete!





